linearity of merge

RunTime/src/MergeSortDirect.lean
@@ -6,6 +6,21 @@ local infix ` ≼ ` : 50 := r
 
 namespace counting
 
+@[simp] def split : list α → (list α × list α × ℕ)
+| []       := ([], [], 0)
+| (a :: l) := let (l₁, l₂, n) := split l in (a :: l₂, l₁, n + 1)
+
+
+theorem length_split_lt {a b} {l l₁ l₂ : list α} {n : ℕ} (h : split (a::b::l) = (l₁, l₂, n)) :
+  list.length l₁ < list.length (a::b::l) ∧ list.length l₂ < list.length (a::b::l) :=
+begin
+  sorry
+  -- cases e : split l with l₁' l₂',
+  -- injection (split_cons_of_eq _ (split_cons_of_eq _ e)).symm.trans h, substs l₁ l₂,
+  -- cases length_split_le e with h₁ h₂,
+  -- exact ⟨nat.succ_le_succ (nat.succ_le_succ h₁), nat.succ_le_succ (nat.succ_le_succ h₂)⟩
+end
+
 def merge : list α → list α → (list α × ℕ)
 | []       l'        := (l', 0)
 | l        []        := (l,  0)
@@ -19,26 +34,45 @@ def merge_sort : list α → (list α × ℕ)
 | []        := ([],  0)
 | [a]       := ([a], 0)
 | (a::b::l) := begin
-  cases e : list.split (a::b::l) with l₁ l₂,
-  cases list.length_split_lt e with h₁ h₂,
+  cases e : split (a::b::l) with l₁ l₂n,
+  cases l₂n with l₂ n,
+  cases length_split_lt e with h₁ h₂,
   cases merge_sort l₁ with l₁' n₁,
   cases merge_sort l₂ with l₂' n₂,
   cases merge r l₁' l₂' with l' m,
-  exact (l', m + n₁ + n₂)
+  exact (l', m + n₁ + n₂ + n)
 end
 using_well_founded {
   rel_tac := λ_ _, `[exact ⟨_, inv_image.wf list.length nat.lt_wf⟩],
   dec_tac := tactic.assumption }
 
+theorem merge_complexity : ∀ l l' : list α , (merge r l l').snd ≤ l.length + l'.length
+| []   []               := begin unfold merge, simp, end
+| []   (h' :: t')       := begin unfold merge, simp, end
+| (h :: t)    []        := begin unfold merge, simp, end
+| (h₁ :: t₁) (h₂ :: t₂) :=
+begin
+  unfold merge, split_ifs,
+  { have hh := merge_complexity t₁ (h₂ :: t₂),
+    cases (merge r t₁ (h₂ :: t₂)),
+    unfold merge,
+    simp at hh,
+    simp,
+    linarith,
+  },
+  { have hh := merge_complexity (h₁ :: t₁) t₂,
+    cases (merge r (h₁ :: t₁) t₂),
+    unfold merge,
+    simp at hh,
+    simp,
+    linarith,
+  }
+end
 
-#eval nat.log 2 8
-
-theorem merge_complexity : ∀ l l' : list α , (merge r l l').snd ≤ min l.length l'.length := sorry
-
-theorem merge_identification : ∀ l l' : list α , (merge r l l').fst = list.merge r l l' := sorry
+theorem merge_equivalence : ∀ l l' : list α , (merge r l l').fst = list.merge r l l' := sorry
 
 theorem merge_sort_complexity : ∀ l : list α , (merge_sort r l).snd ≤ l.length * nat.log 2 l.length := sorry
 
-theorem merge_sort_identification : ∀ l : list α , (merge_sort r l).fst = list.merge_sort r l := sorry
+theorem merge_sort_equivalence : ∀ l : list α , (merge_sort r l).fst = list.merge_sort r l := sorry
 
 end counting
